a test in same file

concurrency/node-replication/InfiniteLog.i.dfy
@@ -1,7 +1,7 @@
 include "../framework/AsyncSSM.s.dfy"
 include "NRSpec.s.dfy"
 include "../../lib/Base/Option.s.dfy"
-
+include "NRSimple.i.dfy"
 
 module InfiniteLogSSM(nrifc: NRIfc) refines TicketStubSSM(nrifc) {
   import opened Options
@@ -488,6 +488,13 @@ module InfiniteLogSSM(nrifc: NRIfc) refines TicketStubSSM(nrifc) {
   }
 
   // constructs the log map with the new entries
+  function{:opaque} F(i:int):int { i + 1 } lemma L() { reveal_F(); assert F(10) == 11; } 
+  lemma bar() {
+    assert F(1)==3;
+    reveal_F();
+  }
+
+
   function  {:opaque}  ConstructNewLogEntries(rids: seq<RequestId>, nodeId: NodeId, gtail: nat, lupd: map<RequestId, UpdateState>): (res: map<nat, LogEntry>)
     requires forall r | r in rids :: r in lupd && lupd[r].UpdateInit?
   {
@@ -1683,3 +1690,623 @@ module InfiniteLogSSM(nrifc: NRIfc) refines TicketStubSSM(nrifc) {
     }
   }
 }
+
+abstract module InfiniteLog_Refines_NRSimple(nrifc: NRIfc) refines
+  Refinement(
+    AsyncIfc(nrifc),
+    TicketStubStateMachine(nrifc, InfiniteLogSSM(nrifc)), // A
+    NRSimple(nrifc) // B
+  )
+{
+  import opened IL = InfiniteLogSSM(nrifc)
+  import opened RequestIds
+   import opened Options
+
+  predicate Inv(s: A.Variables) {
+    IL.Inv(s)
+  }
+
+  lemma InitImpliesInv(s: A.Variables)
+  //requires A.Init(s)
+  ensures Inv(s)
+  {
+    IL.InitImpliesInv(s);
+  }
+
+  lemma NextPreservesInv(s: A.Variables, s': A.Variables, op: ifc.Op)
+  //requires Inv(s)
+  //requires A.Next(s, s', op)
+  ensures Inv(s')
+  {
+    match op {
+      case Start(rid, input) => {
+        IL.NewTicketPreservesInv(s, s', rid, input);
+      }
+      case End(rid, output) => {
+        var stub :| IL.ConsumeStub(s, s', rid, output, stub);
+        IL.ConsumeStubPreservesInv(s, s', rid, output, stub);
+      }
+      case InternalOp => {
+        var shard, shard', rest :| A.InternalNext(s, s', shard, shard', rest);
+        IL.InternalPreservesInv(shard, shard', rest);
+      }
+    }
+  }
+
+  // updates map m1 with map m2, where all values of m2 aree added to m1, and existing values updated
+  // can we just have one definition of this somewhere?
+  // see: https://stackoverflow.com/questions/52610402/updating-a-map-with-another-map-in-dafny
+  function {:opaque} map_update<K(!new), V>(m1: map<K, V>, m2: map<K, V>): map<K, V>
+    ensures forall k :: k in m1 || k in m2 ==> k in map_update(m1, m2)
+    ensures forall k :: k in m2 ==> map_update(m1, m2)[k] == m2[k]
+    ensures forall k :: !(k in m2) && k in m1 ==> map_update(m1, m2)[k] == m1[k]
+    ensures forall k :: !(k in m2) && !(k in m1) ==> !(k in map_update(m1, m2))
+    ensures m1 == map[] ==> map_update(m1, m2) == m2
+    ensures m2 == map[] ==> map_update(m1, m2) == m1
+    ensures (m1.Keys !! m2.Keys) ==> map_update(m1, m2).Keys == m1.Keys + m2.Keys
+    ensures (m1.Keys !! m2.Keys) ==> (forall k | k in m1 :: map_update(m1, m2)[k] == m1[k])
+    ensures (m1.Keys !! m2.Keys) ==> (forall k | k in m2 :: map_update(m1, m2)[k] == m2[k])
+  {
+    map k | k in (m1.Keys + m2.Keys) :: if k in m2 then m2[k] else m1[k]
+  }
+
+  lemma map_update_commutative<K(!new), V>(m1: map<K, V>, m2: map<K, V>)
+    requires m1.Keys !! m2.Keys
+    ensures map_update(m1, m2) == map_update(m2, m1)
+  {
+  }
+
+  lemma map_update_associative<K(!new), V>(m1: map<K, V>, m2: map<K, V>, m3: map<K, V>)
+    requires m1.Keys !! m2.Keys && m2.Keys !! m3.Keys && m3.Keys !! m1.Keys
+    ensures map_update(m1, map_update(m2, m3)) == map_update(map_update(m1, m2), m3)
+  {
+  }
+
+  // construction of the read requests for InfiniteLog -> NRSimple
+  function {:opaque} I_ReadRequests(reqs: map<RequestId, ReadonlyState>) : (res :map<RequestId, B.ReadReq>)
+  {
+    map rid | rid in reqs ::
+      if reqs[rid].ReadonlyInit? then B.ReadInit(reqs[rid].op) else B.ReadReq(reqs[rid].ctail, reqs[rid].op)
+  }
+
+  // predicate to filter in-progress update requests
+  predicate UpdateRequests_InProgress(rid: RequestId, lupd: map<RequestId, UpdateState>)
+  {
+    && rid in lupd
+    && (lupd[rid].UpdateInit? )
+  }
+
+  // construction of the update requests for InfiniteLog -> NRSimple
+  function {:opaque} I_UpdateRequests(lupd: map<RequestId, UpdateState>,  log: map<nat, LogEntry>) : (res : map<RequestId, nrifc.UpdateOp>)
+    requires forall rid | rid in lupd && (lupd[rid].UpdatePlaced? || lupd[rid].UpdateApplied?) :: lupd[rid].idx in log
+  {
+    map rid | rid in lupd && UpdateRequests_InProgress(rid, lupd) ::
+      (if lupd[rid].UpdateInit? then lupd[rid].op else log[lupd[rid].idx].op)
+  }
+
+  // predicate to filter completed update requests
+  predicate UpdateRequests_Done(rid: RequestId, lupd: map<RequestId, UpdateState>)
+  {
+    && rid in lupd
+    && (lupd[rid].UpdateDone? || lupd[rid].UpdatePlaced? || lupd[rid].UpdateApplied?)
+  }
+
+  // construction of the update responses for InfiniteLog -> NRSimple
+  function {:opaque} I_UpdateResponses(lupd: map<RequestId, UpdateState>) : (res : map<RequestId, B.UpdateResp>)
+  {
+    map rid | rid in lupd && UpdateRequests_Done(rid, lupd) :: B.UpdateResp(lupd[rid].idx)
+  }
+
+  function {:opaque} I_Log(gtail: nat, log: map<nat, LogEntry>) : seq<nrifc.UpdateOp>
+    requires forall i | 0 <= i < gtail :: i in log
+  {
+    seq(gtail, i requires 0 <= i < gtail => log[i].op)
+  }
+
+
+  lemma I_Added_LocalRead_is(s: A.Variables, s': A.Variables, rid: RequestId, input: nrifc.Input)
+    requires Inv(s)
+    requires input.ROp?
+    requires s' == s.(localReads := s.localReads[rid := ReadonlyInit(input.readonly_op)])
+    ensures I(s') == I(s).(readonly_reqs := I(s).readonly_reqs[rid := B.ReadInit(input.readonly_op)])
+  {
+    reveal_I_ReadRequests();
+    assert I(s').readonly_reqs == I(s).readonly_reqs[rid := B.ReadInit(input.readonly_op)];
+  }
+
+  lemma I_Removed_LocalReads_is(s: A.Variables, s': A.Variables, rid: RequestId)
+    requires Inv(s)
+    requires s' == s.(localReads := s.localReads - {rid})
+    ensures I(s') == I(s).(readonly_reqs := I(s).readonly_reqs - {rid})
+  {
+    reveal_I_ReadRequests();
+    assert I(s').readonly_reqs == I(s).readonly_reqs - {rid};
+  }
+
+  lemma I_LocalReads_CtailRead(s: A.Variables, s': A.Variables, rid: RequestId, op: nrifc.ReadonlyOp)
+    requires Inv(s)
+    requires s' == s.(localReads := s.localReads[rid := ReadonlyCtail(op, s.ctail.value)])
+    ensures I(s') == I(s).(readonly_reqs := I(s).readonly_reqs[rid := B.ReadReq(I(s).ctail, op)])
+  {
+    reveal_I_ReadRequests();
+    assert I(s').readonly_reqs == I(s).readonly_reqs[rid := B.ReadReq(I(s).ctail, op)];
+  }
+
+  lemma I_LocalReads_ReadOnlyDone(s: A.Variables, s': A.Variables, rid: RequestId, ret: nrifc.ReturnType)
+    requires Inv(s)
+    requires Inv(s')
+    requires rid in s.localReads && s.localReads[rid].ReadonlyReadyToRead?
+    requires s' == s.(localReads := s.localReads[rid := ReadonlyDone(s.localReads[rid].op, ret, s.localReads[rid].ctail)])
+    ensures I(s').readonly_reqs == I(s).readonly_reqs
+  {
+    reveal_I_ReadRequests();
+  }
+
+  lemma I_Removed_LocalUpdates_is(s: A.Variables, s': A.Variables, rid: RequestId)
+    requires Inv(s)
+    requires s' == s.(localUpdates := s.localUpdates - {rid})
+    requires rid in s.localUpdates && s.localUpdates[rid].UpdateDone?
+    ensures I(s') == I(s).(update_resps := I(s).update_resps - {rid})
+  {
+    reveal_I_UpdateRequests();
+    assert I(s').update_reqs == I(s).update_reqs;
+    reveal_I_UpdateResponses();
+    assert I(s').update_resps == I(s).update_resps - {rid};
+  }
+
+  lemma I_Added_LocalUpdate_is(s: A.Variables, s': A.Variables, rid: RequestId, input: nrifc.Input)
+    requires Inv(s)
+    requires rid !in s.localUpdates;
+    requires input.UOp?
+    requires s' == s.(localUpdates := s.localUpdates[rid := UpdateInit(input.update_op)])
+    ensures I(s') == I(s).(update_reqs := I(s).update_reqs[rid := input.update_op])
+  {
+    reveal_I_UpdateRequests();
+    assert I(s').update_reqs == I(s).update_reqs[rid := input.update_op];
+    reveal_I_UpdateResponses();
+    assert I(s').update_resps == I(s).update_resps;
+  }
+
+  lemma I_LocalUpdates_UpdateApplied(lupd: map<RequestId, UpdateState>, lupd': map<RequestId, UpdateState>, log: map<nat, LogEntry>, rid: RequestId, idx: nat, ret: nrifc.ReturnType)
+    requires lupd' == lupd[rid := UpdateApplied(ret, idx)];
+    requires rid in lupd && lupd[rid].UpdatePlaced? && lupd[rid].idx == idx;
+
+    // to make I_Update_Responses Happy
+    requires forall rid | rid in lupd && (lupd[rid].UpdatePlaced? || lupd[rid].UpdateApplied?) :: lupd[rid].idx in log
+    requires forall rid | rid in lupd && (lupd'[rid].UpdatePlaced? || lupd'[rid].UpdateApplied?) :: lupd'[rid].idx in log
+    ensures I_UpdateResponses(lupd) == I_UpdateResponses(lupd')
+    ensures I_UpdateRequests(lupd, log) == I_UpdateRequests(lupd', log)
+  {
+    assert I_UpdateResponses(lupd) == I_UpdateResponses(lupd') by {
+      reveal_I_UpdateResponses();
+    }
+
+    assert I_UpdateRequests(lupd, log) == I_UpdateRequests(lupd', log) by {
+      reveal_I_UpdateRequests();
+    }
+  }
+
+  lemma I_LocalUpdates_UpdateDone(s: A.Variables, s': A.Variables, rid: RequestId, idx: nat, ret: nrifc.ReturnType)
+    requires Inv(s)
+    requires Inv(s')
+    requires rid in s.localUpdates && s.localUpdates[rid].UpdateApplied?
+    requires s' == s.(localUpdates := s.localUpdates[rid:= UpdateDone(ret, idx)]);
+    ensures I(s').update_reqs == I(s).update_reqs - {rid};
+    ensures I(s').update_resps == I(s).update_resps[rid := B.UpdateResp(idx)];
+  {
+      assert I(s').update_reqs == I(s).update_reqs - {rid} by {
+        reveal_I_UpdateRequests();
+      }
+      assert I(s').update_resps == I(s).update_resps[rid := B.UpdateResp(idx)] by {
+        reveal_I_UpdateResponses();
+      }
+  }
+
+
+
+  function I(s: A.Variables) : B.Variables
+  //requires Inv(s)
+  {
+    B.Variables(
+      I_Log(s.global_tail.value, s.log),
+      // [], Inv_LogEntriesGlobalTail
+      s.ctail.value,
+      // readonly_reqs - ReadReq(ctail_at_start: nat, op: nrifc.ReadonlyOp)
+      // TODO(travis): change NRCtail so it has states without ctail (corresponds to NrInfinite)
+      I_ReadRequests(s.localReads),
+      // update_reqs - UpdateResp(idx_in_log: nat, ret: nrifc.ReturnType)
+      I_UpdateRequests(s.localUpdates, s.log),
+      // update_resps - UpdateResp(idx_in_log: nat, ret: nrifc.ReturnType)
+      I_UpdateResponses(s.localUpdates)
+    )
+  }
+
+  lemma InitRefinesInit(s: A.Variables)
+  //requires A.Init(s)
+  //requires Inv(s)
+  ensures B.Init(I(s))
+
+
+
+  lemma NewTicket_Refines_Start_LocalReads(s: A.Variables, s': A.Variables,
+                                           rid: RequestId, input: nrifc.Input)
+    requires IL.NewTicket(s, s', rid, input)
+    requires s.M?
+    requires input.ROp?;
+    ensures s' == s.(localReads := s.localReads[rid := ReadonlyInit(input.readonly_op)])
+  {
+  }
+
+  lemma NewTicket_Refines_Start_LocalUpdates(s: A.Variables, s': A.Variables,
+                                             rid: RequestId, input: nrifc.Input)
+    requires IL.NewTicket(s, s', rid, input)
+    requires s.M?
+    requires input.UOp?
+    ensures s' == s.(localUpdates := s.localUpdates[rid := UpdateInit(input.update_op)])
+  {
+  }
+
+  // s: some previous thing with a missing piece
+  // s': some next thing
+  // "stub": the missing piece in s
+  // s' = s + ticket
+  lemma NewTicket_Refines_Start(s: A.Variables, s': A.Variables,
+      rid: RequestId, input: nrifc.Input)
+  requires IL.NewTicket(s, s', rid, input)
+  requires Inv(s)
+  requires Inv(s')
+  ensures B.Next(I(s), I(s'), ifc.Start(rid, input))
+  {
+    // checks, but may take a bit long....
+    assume false;
+
+    // construct the ticket
+    if input.ROp? {
+      assert I(s') == I(s).(readonly_reqs := I(s).readonly_reqs[rid := B.ReadInit(input.readonly_op)]) by {
+        NewTicket_Refines_Start_LocalReads(s, s', rid, input);
+        I_Added_LocalRead_is(s, s', rid, input);
+      }
+
+      assert exists step :: B.NextStep(I(s), I(s'), ifc.Start(rid, input), step) by {
+        var step := B.StartReadonly_Step(rid, input.readonly_op);
+        assert B.NextStep(I(s), I(s'), ifc.Start(rid, input), step) by {
+          assert B.StartReadonly(I(s), I(s'), rid,  input.readonly_op);
+        }
+      }
+
+    } else {
+      assert rid !in s.localUpdates;
+      assert input.UOp?;
+      // proves but takes a while
+      assert I(s') == I(s).(update_reqs := I(s).update_reqs[rid := input.update_op]) by {
+        NewTicket_Refines_Start_LocalUpdates(s, s', rid, input);
+        I_Added_LocalUpdate_is(s, s', rid, input);
+      }
+
+      assert exists step :: B.NextStep(I(s), I(s'), ifc.Start(rid, input), step) by {
+        var step := B.StartUpdate_Step(rid, input.update_op);
+        assert B.NextStep(I(s), I(s'), ifc.Start(rid, input), step) by {
+          assert B.StartUpdate(I(s), I(s'), rid,  input.update_op);
+        }
+      }
+    }
+  }
+
+  lemma ConsumeStub_Refines_End_LocalReads(s: A.Variables, s': A.Variables,
+      rid: RequestId, output: nrifc.Output, stub: M)
+    requires IL.ConsumeStub(s, s', rid, output, stub)
+    requires rid in stub.localReads
+    requires s.M?
+    ensures s' == s.(localReads := s.localReads - {rid})
+  {
+  }
+
+  lemma ConsumeStub_Refines_End_LocalUpdates(s: A.Variables, s': A.Variables,
+      rid: RequestId, output: nrifc.Output, stub: M)
+    requires IL.ConsumeStub(s, s', rid, output, stub)
+    requires rid in stub.localUpdates
+    requires s.M?
+    ensures s' == s.(localUpdates := s.localUpdates - {rid})
+  {
+  }
+
+  predicate VersionInLog(log: map<nat, LogEntry>, version: nat)
+  {
+    forall i | 0 <= i < version :: i in log
+  }
+
+  predicate OutputMatch(log: map<nat, LogEntry>,  output: nrifc.Output, version: nat, op: nrifc.ReadonlyOp)
+    requires VersionInLog(log, version)
+  {
+     output == nrifc.read(state_at_version(log, version), op)
+  }
+
+  lemma ConsumeStub_Refines_End(s: A.Variables, s': A.Variables,
+      rid: RequestId, output: nrifc.Output, stub: M)
+  requires IL.ConsumeStub(s, s', rid, output, stub)
+  requires Inv(s)
+  requires Inv(s')
+  ensures B.Next(I(s), I(s'), ifc.End(rid, output))
+  {
+    if rid in stub.localUpdates {
+
+      assert I(s') == I(s).(update_resps := I(s).update_resps - {rid}) by {
+        ConsumeStub_Refines_End_LocalUpdates(s, s', rid, output, stub);
+        I_Removed_LocalUpdates_is(s, s', rid);
+      }
+
+      assert stub.localUpdates[rid].ret == output;
+      assert s.localUpdates[rid].ret == output;
+      // assert s.localUpdates[rid].ret == nrifc.update(state_at_version(s.log, idx), s.log[idx]).return_value;
+
+      assert exists step :: B.NextStep(I(s), I(s'), ifc.End(rid, output), step) by {
+        var step := B.EndUpdate_Step(rid, output);
+        assert B.NextStep(I(s), I(s'), ifc.End(rid, output), step) by {
+          // that one now taks a bit longer, due to the return value that we now construct in the EndUpdate?
+          assume false;
+          assert B.EndUpdate(I(s), I(s'), rid,  output);
+        }
+      }
+
+    } else {
+
+      assert rid in stub.localReads;
+      assert rid in s.localReads;
+
+      assert I(s') == I(s).(readonly_reqs := I(s).readonly_reqs - {rid}) by {
+        ConsumeStub_Refines_End_LocalReads(s, s', rid, output, stub);
+        I_Removed_LocalReads_is(s, s', rid);
+      }
+      assert exists step :: B.NextStep(I(s), I(s'), ifc.End(rid, output), step) by {
+
+        assume exists version : nat | version <= s.ctail.value :: VersionInLog(s.log, version) && OutputMatch(s.log, output, version,  s.localReads[rid].op);
+        var version : nat :| version <= s.ctail.value  && VersionInLog(s.log, version) && OutputMatch(s.log, output, version,  s.localReads[rid].op);
+
+        var step := B.FinishReadonly_Step(rid, version, output);
+
+        assert rid in I(s).readonly_reqs by {
+          reveal_I_ReadRequests();
+        }
+
+        assert I(s).readonly_reqs[rid].ReadReq? by {
+          assert s.localReads[rid].ReadonlyDone?;
+           reveal_I_ReadRequests();
+        }
+
+        assert I(s).readonly_reqs[rid].ctail_at_start <= version <= |I(s).log| by {
+          assume false;
+        }
+
+        assert output == nrifc.read(B.state_at_version(I(s).log, version), I(s).readonly_reqs[rid].op) by {
+          assume false;
+        }
+
+         assert B.NextStep(I(s), I(s'), ifc.End(rid, output), step) by {
+           assert B.FinishReadonly(I(s), I(s'), rid, version, output) by {
+            assert version <= I(s).ctail;
+
+
+           }
+         }
+      }
+    }
+  }
+
+  lemma GoToCombinerReady_Refines(s: A.Variables, s': A.Variables, nodeId: IL.NodeId)
+  requires IL.GoToCombinerReady(s, s', nodeId)
+  requires Inv(s)
+  requires Inv(s')
+  ensures B.Next(I(s), I(s'), ifc.InternalOp)
+  {
+    assert B.NextStep(I(s), I(s'), ifc.InternalOp, B.Stutter_Step);
+  }
+
+  lemma ExecLoadLtail_Refines(s: A.Variables, s': A.Variables, nodeId: IL.NodeId)
+  requires IL.ExecLoadLtail(s, s', nodeId)
+  requires Inv(s)
+  requires Inv(s')
+  ensures B.Next(I(s), I(s'), ifc.InternalOp)
+  {
+    assert B.NextStep(I(s), I(s'), ifc.InternalOp, B.Stutter_Step);
+  }
+
+  lemma ExecLoadGlobalTail_Refines(s: A.Variables, s': A.Variables, nodeId: IL.NodeId)
+  requires IL.ExecLoadGlobalTail(s, s', nodeId)
+  requires Inv(s)
+  requires Inv(s')
+  ensures B.Next(I(s), I(s'), ifc.InternalOp)
+  {
+    assert B.NextStep(I(s), I(s'), ifc.InternalOp, B.Stutter_Step);
+  }
+
+  lemma ExecDispatchLocal_Refines(s: A.Variables, s': A.Variables, nodeId: IL.NodeId)
+  requires IL.ExecDispatchLocal(s, s', nodeId)
+  requires Inv(s)
+  requires Inv(s')
+  ensures B.Next(I(s), I(s'), ifc.InternalOp)
+  {
+    var c := s.combiner[nodeId];
+    var UpdateResult(nr_state', ret) := nrifc.update(s.replicas[nodeId], s.log[c.localTail].op);
+    var queue_index := |c.queued_ops| - (c.globalTail - c.localTail);
+    var request_id := c.queued_ops[queue_index];
+    var idx :=  s.localUpdates[request_id].idx;
+
+    I_LocalUpdates_UpdateApplied(s.localUpdates, s'.localUpdates, s.log, request_id, idx, ret);
+    assert B.NextStep(I(s), I(s'), ifc.InternalOp, B.Stutter_Step);
+  }
+
+  lemma ExecDispatchRemote_Refines(s: A.Variables, s': A.Variables, nodeId: IL.NodeId)
+  requires IL.ExecDispatchRemote(s, s', nodeId)
+  requires Inv(s)
+  requires Inv(s')
+  ensures B.Next(I(s), I(s'), ifc.InternalOp)
+  {
+    assert B.NextStep(I(s), I(s'), ifc.InternalOp, B.Stutter_Step);
+  }
+
+  lemma TransitionReadonlyReadCtail_Refines(s: A.Variables, s': A.Variables, nodeId: IL.NodeId, rid: RequestId)
+  requires IL.TransitionReadonlyReadCtail(s, s', nodeId, rid)
+  requires Inv(s)
+  requires Inv(s')
+  ensures B.Next(I(s), I(s'), ifc.InternalOp)
+  {
+
+    var op := s.localReads[rid].op;
+
+    assert rid in I(s).readonly_reqs && I(s).readonly_reqs[rid].ReadInit? by {
+      reveal_I_ReadRequests();
+    }
+
+    assert op == I(s).readonly_reqs[rid].op by {
+      reveal_I_ReadRequests();
+    }
+
+    assert s' == s.(localReads := s.localReads[rid := ReadonlyCtail(op, s.ctail.value)]);
+    I_LocalReads_CtailRead(s, s', rid, op);
+    assert B.NextStep(I(s), I(s'), ifc.InternalOp, B.ReadCtail_Step(rid));
+  }
+
+  lemma TransitionReadonlyReadyToRead_Refines(s: A.Variables, s': A.Variables, nodeId: IL.NodeId, rid: RequestId)
+  requires IL.TransitionReadonlyReadyToRead(s, s', nodeId, rid)
+  requires Inv(s)
+  requires Inv(s')
+  ensures B.Next(I(s), I(s'), ifc.InternalOp)
+  {
+    var IS := I(s);
+    var IS' := I(s');
+
+    var r := s.localReads[rid];
+    assert s' == s.(localReads := s.localReads[rid := ReadonlyReadyToRead(r.op, nodeId, r.ctail)]);
+    assert s'.localReads[rid].op == s.localReads[rid].op;
+    assert s'.localReads[rid].ctail == s.localReads[rid].ctail;
+
+    assert IS.ctail == IS'.ctail && IS.ctail == s.ctail.value;
+    assert IS.log == IS'.log;
+
+    assert IS.update_resps == IS'.update_resps;
+    assert IS.update_reqs == IS'.update_reqs;
+    reveal_I_ReadRequests();
+    assert IS'.readonly_reqs == IS.readonly_reqs;
+    // no corresponding step
+    assert B.NextStep(I(s), I(s'), ifc.InternalOp, B.Stutter_Step);
+  }
+
+  lemma TransitionReadonlyDone_Refines(s: A.Variables, s': A.Variables, nodeId: IL.NodeId, rid: RequestId)
+  requires IL.TransitionReadonlyDone(s, s', nodeId, rid)
+  requires Inv(s)
+  requires Inv(s')
+  ensures B.Next(I(s), I(s'), ifc.InternalOp)
+  {
+    var req := s.localReads[rid];
+    var ret := nrifc.read(s.replicas[req.nodeId], req.op);
+    I_LocalReads_ReadOnlyDone(s, s', rid, ret);
+    assert B.NextStep(I(s), I(s'), ifc.InternalOp,  B.Stutter_Step);
+  }
+
+  // lemma AdvanceTail_Refines_foo(s: A.Variables, s': A.Variables, nodeId: IL.NodeId, request_ids: seq<RequestId>)
+  //   requires s'.localUpdates == map_update(s.localUpdates, local_updates_new)
+  //   requires Inv(s)
+  //   requires Inv(s')
+  //   ensures
+
+  lemma AdvanceTail_Refines(s: A.Variables, s': A.Variables, nodeId: IL.NodeId, request_ids: seq<RequestId>)
+  requires IL.AdvanceTail(s, s', nodeId, request_ids)
+  requires Inv(s)
+  requires Inv(s')
+  ensures B.Next(I(s), I(s'), ifc.InternalOp)
+  {
+    assert F(1)==3;
+    reveal_F();
+  
+
+    // that on takes a bit...?
+    var new_log_entries := B.ConstructNewLogEntries(request_ids, I(s).update_reqs);
+//     assume I(s').log == I(s).log + new_log_entries;
+
+    //assert B.RequestIdsValid(request_ids, I(s).update_reqs);
+
+    // construct the responses
+
+
+
+    //assume B.AddUpdateToLog(I(s), I(s'), request_ids);
+
+    assume false;
+    assert exists step :: B.NextStep(I(s), I(s'), ifc.InternalOp, step) by {
+    //   var step :=
+      assert B.NextStep(I(s), I(s'), ifc.InternalOp, B.AddUpdateToLog_Step(request_ids)) by {
+        assume B.AddUpdateToLog(I(s), I(s'), request_ids);
+      }
+    }
+
+  }
+
+  lemma UpdateCompletedTail_Refines(s: A.Variables, s': A.Variables, nodeId: IL.NodeId)
+  requires IL.UpdateCompletedTail(s, s', nodeId)
+  requires Inv(s)
+  requires Inv(s')
+  ensures B.Next(I(s), I(s'), ifc.InternalOp)
+  {
+    var c := s.combiner[nodeId];
+    var new_ctail := if s.ctail.value > c.localTail then s.ctail.value else c.localTail;
+    assert B.NextStep(I(s), I(s'), ifc.InternalOp, B.IncreaseCtail_Step(new_ctail));
+  }
+
+  lemma UpdateRequestDone_Refines(s: A.Variables, s': A.Variables, rid: RequestId)
+  requires IL.UpdateRequestDone(s, s', rid)
+  requires Inv(s)
+  requires Inv(s')
+  ensures B.Next(I(s), I(s'), ifc.InternalOp)
+  {
+    var req := s.localUpdates[rid];
+    assert s' == s.(localUpdates := s.localUpdates[rid:= UpdateDone(req.ret, req.idx)]);
+    I_LocalUpdates_UpdateDone(s, s', rid, req.idx, req.ret);
+
+    assert B.NextStep(I(s), I(s'), ifc.InternalOp, B.Stutter_Step);
+  }
+
+  lemma Internal_Refines_Internal(s: A.Variables, s': A.Variables)
+  requires IL.Internal(s, s')
+  requires Inv(s)
+  requires Inv(s')
+  ensures B.Next(I(s), I(s'), ifc.InternalOp)
+  {
+    var step :| NextStep(s, s', step);
+    match step {
+      case GoToCombinerReady_Step(nodeId) => { GoToCombinerReady_Refines(s, s', nodeId); }
+      case ExecLoadLtail_Step(nodeId) => { ExecLoadLtail_Refines(s, s', nodeId); }
+      case ExecLoadGlobalTail_Step(nodeId) => { ExecLoadGlobalTail_Refines(s, s', nodeId); }
+      case ExecDispatchLocal_Step(nodeId) => { ExecDispatchLocal_Refines(s, s',nodeId); }
+      case ExecDispatchRemote_Step(nodeId) => { ExecDispatchRemote_Refines(s, s',nodeId); }
+      case TransitionReadonlyReadCtail_Step(nodeId, rid) => { TransitionReadonlyReadCtail_Refines(s, s', nodeId, rid); }
+      case TransitionReadonlyReadyToRead_Step(nodeId, rid) => { TransitionReadonlyReadyToRead_Refines(s, s', nodeId, rid); }
+      case TransitionReadonlyDone_Step(nodeId, rid) => { TransitionReadonlyDone_Refines(s, s', nodeId, rid); }
+      case AdvanceTail_Step(nodeId, request_ids) => { AdvanceTail_Refines(s, s', nodeId, request_ids); }
+      case UpdateCompletedTail_Step(nodeId) => { UpdateCompletedTail_Refines(s, s',nodeId); }
+      case UpdateRequestDone_Step(request_id: RequestId) => { UpdateRequestDone_Refines(s, s', request_id); }
+    }
+  }
+
+  lemma NextRefinesNext(s: A.Variables, s': A.Variables, op: ifc.Op)
+  //requires Inv(s)
+  //requires Inv(s')
+  //requires A.Next(s, s', op)
+  ensures B.Next(I(s), I(s'), op)
+  {
+    match op {
+      case Start(rid, input) => {
+        NewTicket_Refines_Start(s, s', rid, input);
+      }
+      case End(rid, output) => {
+        var stub :| IL.ConsumeStub(s, s', rid, output, stub);
+        ConsumeStub_Refines_End(s, s', rid, output, stub);
+      }
+      case InternalOp => {
+        var shard, shard', rest :| A.InternalNext(s, s', shard, shard', rest);
+        InternalMonotonic(shard, shard', rest);
+        Internal_Refines_Internal(s, s');
+      }
+    }
+  }
+}
+
